update erc20 - dafny

dafny/src/erc20.dfy
@@ -2,11 +2,13 @@
 include "util/number.dfy"
 include "util/maps.dfy"
 include "util/tx.dfy"
+include "util/fixed.dfy"
 
 
 import opened Number
 import opened Maps
 import opened Tx
+import opened Fixed
 
 
 class ERC20 {
@@ -16,18 +18,17 @@ class ERC20 {
     var allowance: mapping<u160, mapping<u160,u256>>
     var supply: u256
 
-    var fee: u256
+    const fee: u256 := 3
+    const WAD: u256 := 1_000_000_000_000_000_000
 
     var owner: u160
 
-    constructor(ownerAddress: u160) {
+    constructor() {
         balances := Map(map[], 0);
         allowance := Map(map[], Map(map[],0));
         supply := 0;
-
-        fee := 3;
         
-        owner := ownerAddress;
+        // owner := msg.sender;
     }
 
     method fallback(msg: Transaction) returns (r: Result<()>)
@@ -80,8 +81,8 @@ class ERC20 {
     }
 
     method calculateFee(wad: u256) returns (calcFee: u256)
-    requires wad as nat * fee as nat <= MAX_U256 as nat {
-        calcFee := (wad * fee) / 100;
+    requires (fee / 100) != 0 {
+        calcFee := Wdiv(wad, Wdiv(fee, 100));
     }
 
 
@@ -91,13 +92,15 @@ class ERC20 {
     requires this.balances.default == 0
     requires msg.sender in balances.Keys()
     requires dst in balances.Keys()
-    requires wad as nat * fee as nat <= MAX_U256 as nat
+    requires (fee / 100) != 0
     requires msg.value == 0 {  // non-payable
-        r := transferFrom(msg, msg.sender, dst, wad);
-        var calcFee := calculateFee(wad);
+        var calcWad := calculateFee(wad);
+        r := transferFrom(msg, msg.sender, dst, calcWad);
         assume {:axiom} this.balances.default == 0;
         assume {:axiom} msg.sender in balances.Keys();
         assume {:axiom} owner in balances.Keys();
+        assume {:axiom} wad as nat - calcWad as nat >= 0;
+        var calcFee := wad - calcWad;
         r := transferFrom(msg, msg.sender, owner, calcFee);
     }
 
